theory/x64Generator.thy
@@ -1,0 +1,11 @@
+theory x64Generator
+  imports Main
+  x64Semantics x64Syntax rBPFCommType Val Mem 
+
+begin
+
+export_code x64_interp_test in OCaml
+  module_name x64_interp_test file_prefix x64_interp_test
+
+                             
+end
