theory/x64_encode_subl_ri_1.thy
@@ -1,0 +1,109 @@
+theory x64_encode_subl_ri_1
+imports
+  Main
+  rBPFCommType 
+  x64Syntax BitsOpMore BitsOpMore3
+begin
+
+value "(bit (4::int) 1)"
+
+lemma [simp]: "and 7 ((v::u8) >> 3) = 5 \<Longrightarrow> \<not> bit v (Suc (Suc (Suc (Suc 0)))) "
+  apply (simp add: bit_eq_iff Suc3_eq_add_3 )
+  apply (auto simp add: bit_simps)
+  apply (drule_tac x="1" in spec) by simp
+
+lemma [simp]: "and 7 ((v::u8) >> 3) = 5 \<Longrightarrow> bit v (Suc (Suc (Suc (Suc (Suc 0))))) "
+  apply (simp add: bit_eq_iff Suc3_eq_add_3 )
+  apply (auto simp add: bit_simps)
+  apply (drule_tac x="2" in spec) by simp
+
+
+lemma encode_subl_ri_1_subgoal_1: "
+  and 7 ((v::u8) >> 3) = 5 \<Longrightarrow> and 3 (v >> 6) = 3 \<Longrightarrow> n < 8 \<Longrightarrow> bit v n \<Longrightarrow> \<not> bit (192::u8) n \<Longrightarrow> 
+    \<not> bit (40::u8) n \<Longrightarrow> bit (7::u8) n"
+  apply (cases n, simp_all)
+  subgoal for n1 apply (cases n1, simp_all)    
+    subgoal for n2 apply (cases n2, simp_all)
+      subgoal for n3 apply (cases n3, simp_all)
+        subgoal for n4 apply (cases n4, simp_all)
+          subgoal for n5 apply (cases n5, simp_all)
+            subgoal for n6 apply (cases n6, simp_all)
+              done
+            done
+          done
+        done
+      done
+    done
+  done
+
+lemma encode_subl_ri_1_subgoal_2: "
+    and 7 ((v::u8) >> 3) = 5 \<Longrightarrow> and 3 (v >> 6) = 3 \<Longrightarrow> n < 8 \<Longrightarrow> bit v n \<Longrightarrow> \<not> bit (192::u8) n \<Longrightarrow> \<not> bit (40::u8) n \<Longrightarrow> bit (56::u8) n \<Longrightarrow> False"
+  apply (cases n, simp_all)
+  subgoal for n1 apply (cases n1, simp_all)
+    subgoal for n2 apply (cases n2, simp_all)
+      subgoal for n3 apply (cases n3, simp_all)
+        subgoal for n4 apply (cases n4, simp_all)
+            done
+          done
+        done
+      done
+    done      
+
+lemma encode_subl_ri_1_subgoal_3: "
+    and 7 ((v::u8) >> 3) = 5 \<Longrightarrow> and 3 (v >> 6) = 3 \<Longrightarrow> n < 8 \<Longrightarrow> \<not> bit (192::u8) n \<Longrightarrow> bit (40::u8) n \<Longrightarrow> bit v n"
+  apply (cases n, simp_all)
+  subgoal for n1 apply (cases n1, simp_all)
+    subgoal for n2 apply (cases n2, simp_all)
+      subgoal for n3 apply (cases n3, simp_all)
+        subgoal   
+          by (metis bit_0 bit_and_iff bit_iff_odd_drop_bit bit_numeral_Bit1_0 numeral_3_eq_3)
+        subgoal for n4 apply (cases n4, simp_all)
+          subgoal for n5 apply (cases n5, simp_all)
+            done
+            done
+          done
+        done
+      done
+    done      
+
+
+lemma encode_subl_ri_1_subgoal_k:" u8_of_ireg dst = and 7 v \<Longrightarrow>
+    u32_of_u8_list [l ! Suc (Suc pc), l ! (pc + 3), l ! (pc + 4), l ! (pc + 5)] = Some imm \<Longrightarrow>
+    and 7 (v >> 3) = 5 \<Longrightarrow>
+    and 3 (v >> 6) = 3 \<Longrightarrow> v = or 192 (and (or 40 (and (and 7 v) (- 57))) (- 193)) \<and>
+    [l ! Suc (Suc pc), l ! Suc (Suc (Suc pc)), l ! Suc (Suc (Suc (Suc pc))), l ! Suc (Suc (Suc (Suc (Suc pc))))] = u8_list_of_u32 imm"
+  apply (rule conjI)
+
+  subgoal
+    apply (rule bit_eqI)
+    subgoal for n
+      apply (auto simp add: bit_simps)
+      subgoal using encode_subl_ri_1_subgoal_1 by simp
+      subgoal using encode_subl_ri_1_subgoal_2 by simp
+      subgoal using encode_subl_ri_1_subgoal_3 by simp
+      done
+    done
+
+  subgoal
+   using u32_of_u8_list_same
+   by (smt (verit, best) add_2_eq_Suc' add_Suc group_cancel.add2 nat_arith.suc1 nth_Cons_0 numeral_2_eq_2 numeral_3_eq_3 numeral_Bit0 numeral_Bit1 numeral_plus_numeral semiring_norm(5) u32_of_u8_list_def u8_list_of_u32_def ucast32_ucast8_and_255_eq) 
+  done
+
+
+lemma encode_subl_ri_1: "
+    ireg_of_u8 (bitfield_insert_u8 3 (Suc 0) (and 7 (v)) 0) = Some dst \<Longrightarrow>
+    u32_of_u8_list [l ! Suc (Suc pc), l ! (pc + 3), l ! (pc + 4), l ! (pc + 5)] = Some imm \<Longrightarrow>
+    and 7 (v >> 3) = 5 \<Longrightarrow> and 3 (v >> 6) = 3 \<Longrightarrow>
+    bitfield_insert_u8 4 4
+     (bitfield_insert_u8 3 (Suc 0)
+       (bitfield_insert_u8 2 (Suc 0) (bitfield_insert_u8 (Suc 0) (Suc 0) (u8_of_bool (and (u8_of_ireg dst) 8 \<noteq> 0)) 0) 0) 0)
+     4 =
+    64 \<Longrightarrow>
+    v = bitfield_insert_u8 6 2 (bitfield_insert_u8 3 3 (and 7 (u8_of_ireg dst)) 5) 3 \<and>
+    [l ! Suc (Suc pc), l ! Suc (Suc (Suc pc)), l ! Suc (Suc (Suc (Suc pc))), l ! Suc (Suc (Suc (Suc (Suc pc))))] = u8_list_of_u32 imm"
+  apply (simp add: u8_of_ireg_of_u8_iff[symmetric])
+  apply (unfold bitfield_insert_u8_def Let_def u8_of_bool_def)
+  apply simp
+  using encode_subl_ri_1_subgoal_k by simp
+
+end
