theory/x64_encode_subl_ri_3.thy
@@ -1,0 +1,176 @@
+theory x64_encode_subl_ri_3
+  imports
+  Main
+  rBPFCommType 
+  x64Syntax BitsOpMore BitsOpMore3
+
+
+begin
+
+lemma encode_subl_ri_4_subgoal_1:"and 15 ((v::u8) >> 4) = 4 \<Longrightarrow> and 15 v \<noteq> 0 \<Longrightarrow> \<not> bit v 2 \<Longrightarrow> \<not> bit v (Suc 0) \<Longrightarrow>
+    \<not> bit v 3  \<Longrightarrow> bit v 0  \<Longrightarrow> n < 8 \<Longrightarrow> bit v n = bit (65::int) n"
+  apply (cases n, simp_all)
+  subgoal for n1 apply (cases n1, simp_all)
+    subgoal for n2 apply (cases n2, simp_all)
+      subgoal
+        by (metis numeral_2_eq_2) 
+      subgoal for n3 apply (cases n3, simp_all)
+        subgoal
+          by (metis numeral_3_eq_3)
+        subgoal for n4 apply (cases n4, simp_all)
+          subgoal
+            by (metis add_2_eq_Suc' bit_1_0 bit_and_iff bit_numeral_Bit1_0 bit_word_iff_drop_bit_and not_bit_numeral_Bit0_0 numeral_2_eq_2 numeral_Bit0)
+          subgoal for n5 apply (cases n5, simp_all)
+            subgoal for n6 apply (cases n6, simp_all)
+              done
+            done
+          done
+        done
+      done
+    done
+  done
+
+lemma encode_subl_ri_4_subgoal_2_1 [simp]:"and 7 ((k::u8) >> 3) = 5 \<Longrightarrow>bit k (Suc (Suc (Suc (Suc 0)))) \<Longrightarrow> False"
+  apply (simp add: bit_eq_iff Suc3_eq_add_3)
+  apply (auto simp add: bit_simps)
+  apply (drule_tac x="1" in spec) by simp
+
+
+                                                     
+lemma encode_subl_ri_4_subgoal_2:"
+    and 3 ((k::u8) >> 6) = 3 \<Longrightarrow>
+    and 7 (k >> 3) = 5  \<Longrightarrow> n < 8 \<Longrightarrow> bit k n \<Longrightarrow> \<not> bit (192::u8) n \<Longrightarrow> \<not> bit (40::u8) n \<Longrightarrow> bit (7::u8) n
+"
+  apply (cases n, simp_all)
+  subgoal for n1 apply (cases n1, simp_all) 
+    subgoal for n2 apply (cases n2, simp_all)
+      subgoal for n3 apply (cases n3, simp_all)
+        subgoal for n4 apply (cases n4, simp_all)
+          subgoal using encode_subl_ri_4_subgoal_2_1 by blast
+          subgoal for n5 apply (cases n5, simp_all)
+            subgoal for n6 apply (cases n6, simp_all)
+              done
+            done
+          done
+        done
+      done
+    done
+  done
+
+lemma encode_subl_ri_4_subgoal_3:"
+    and 3 ((k::u8) >> 6) = 3 \<Longrightarrow> and 7 (k >> 3) = 5 \<Longrightarrow> n < 8 \<Longrightarrow> bit k n \<Longrightarrow> \<not> bit (192::u8) n \<Longrightarrow> \<not> bit (40::u8) n \<Longrightarrow> bit (56::u8) n \<Longrightarrow> False
+
+"
+  apply (cases n, simp_all)
+  subgoal for n1 apply (cases n1, simp_all) 
+    subgoal for n2 apply (cases n2, simp_all)
+      subgoal for n3 apply (cases n3, simp_all) 
+        subgoal for n4 apply (cases n4, simp_all)
+          subgoal using encode_subl_ri_4_subgoal_2_1 by blast
+            done
+          done
+        done
+      done
+    done
+
+lemma encode_subl_ri_4_subgoal_3_1 [simp] :" and 7 ((k::u8) >> 3) = 5 \<Longrightarrow> bit k (Suc (Suc (Suc 0)))"
+  apply (simp add: bit_eq_iff Suc3_eq_add_3)
+  apply (auto simp add: bit_simps)
+  done
+
+lemma encode_subl_ri_4_subgoal_3_2 [simp] :" and 7 ((k::u8) >> 3) = 5 \<Longrightarrow> bit k (Suc (Suc (Suc (Suc (Suc 0)))))"
+  apply (simp add: bit_eq_iff Suc3_eq_add_3)
+  apply (auto simp add: bit_simps)
+  apply (drule_tac x="6" in spec) by simp
+  done
+
+
+lemma encode_subl_ri_4_subgoal_4 :"
+    and 3 ((k::u8) >> 6) = 3 \<Longrightarrow> and 7 (k >> 3) = 5 \<Longrightarrow> n < 8 \<Longrightarrow> \<not> bit (192::u8) n \<Longrightarrow> bit (40::u8) n \<Longrightarrow> bit k n
+"
+  apply (cases n, simp_all)
+  subgoal for n1 apply (cases n1, simp_all) 
+    subgoal for n2 apply (cases n2, simp_all)
+      subgoal for n3 apply (cases n3, simp_all) 
+        subgoal for n4 apply (cases n4, simp_all)
+          subgoal for n5 apply (cases n5, simp_all)
+
+          subgoal using encode_subl_ri_4_subgoal_2_1 by blast
+
+
+lemma encode_subl_ri_4_subgoal_k:"
+    and 15 (v >> 4) = 4 \<Longrightarrow> and 15 v \<noteq> 0 \<Longrightarrow>
+    and 3 (k >> 6) = 3 \<Longrightarrow> and 7 (k >> 3) = 5 \<Longrightarrow>
+    u8_of_ireg dst = or (and 8 (v << 3)) (and 7 k) \<Longrightarrow>
+    u32_of_u8_list [l ! (pc + 3), l ! (pc + 4), l ! (pc + 5), l ! (pc + 6)] = Some imm \<Longrightarrow>
+    \<not> bit v 3 \<Longrightarrow> \<not> bit v 2 \<Longrightarrow> \<not> bit v (Suc 0) \<Longrightarrow>
+    or 64 (and (and (and (and (case bit v 0 of True \<Rightarrow> 1 | False \<Rightarrow> 0) (- 3)) (- 5)) (- 9)) (- 241)) \<noteq> 64 \<Longrightarrow>
+    v = or 64 (and (and (and (and (case bit v 0 of True \<Rightarrow> 1 | False \<Rightarrow> 0) (- 3)) (- 5)) (- 9)) (- 241)) \<and>
+    k = or 192 (and (or 40 (and (and 7 (or (and 8 (v << 3)) (and 7 k))) (- 57))) (- 193)) \<and>
+    [l ! Suc (Suc (Suc pc)), l ! Suc (Suc (Suc (Suc pc))), l ! Suc (Suc (Suc (Suc (Suc pc)))),
+     l ! Suc (Suc (Suc (Suc (Suc (Suc pc)))))] = u8_list_of_u32 imm
+"
+  apply (rule conjI)
+  subgoal 
+    apply(cases "bit v 0", simp_all)
+    subgoal
+      apply (rule bit_eqI)
+      subgoal for n
+        apply (auto simp add: bit_simps)
+        subgoal using encode_subl_ri_4_subgoal_1 by blast
+        subgoal using encode_subl_ri_4_subgoal_1 by blast
+        done
+      done
+    done
+
+  apply (rule conjI)
+  subgoal 
+    apply(cases "bit v 0", simp_all)
+    subgoal
+      apply (rule bit_eqI)
+      subgoal for n
+        apply (auto simp add: bit_simps)
+        subgoal 
+          using encode_subl_ri_4_subgoal_2
+          using bit_numeral_word_iff by blast
+        subgoal
+          using \<open>\<lbrakk>and 15 (v >> 4) = 4; and 15 v \<noteq> 0; and 3 (k >> 6) = 3; and 7 (k >> 3) = 5; u8_of_ireg dst = or (and 8 (v << 3)) (and 7 k); u32_of_u8_list [l ! (pc + 3), l ! (pc + 4), l ! (pc + 5), l ! (pc + 6)] = Some imm; \<not> bit v 3; \<not> bit v 2; \<not> bit v (Suc 0); or 64 (and (and (and (and 1 (- 3)) (- 5)) (- 9)) (- 241)) \<noteq> 64; bit v 0; n < 8; bit k n; \<not> bit 192 n; \<not> bit 40 n\<rbrakk> \<Longrightarrow> bit 7 n\<close> by blast
+        subgoal
+          using \<open>\<lbrakk>and 15 (v >> 4) = 4; and 15 v \<noteq> 0; and 3 (k >> 6) = 3; and 7 (k >> 3) = 5; u8_of_ireg dst = or (and 8 (v << 3)) (and 7 k); u32_of_u8_list [l ! (pc + 3), l ! (pc + 4), l ! (pc + 5), l ! (pc + 6)] = Some imm; \<not> bit v 3; \<not> bit v 2; \<not> bit v (Suc 0); or 64 (and (and (and (and 1 (- 3)) (- 5)) (- 9)) (- 241)) \<noteq> 64; bit v 0; n < 8; bit k n; \<not> bit 192 n; \<not> bit 40 n\<rbrakk> \<Longrightarrow> bit 7 n\<close> by fastforce
+        subgoal 
+          using encode_subl_ri_4_subgoal_3 by (meson bit_numeral_word_iff encode_subl_ri_4_subgoal_2)
+        subgoal 
+          using encode_subl_ri_4_subgoal_4
+        done
+      done
+    done
+
+  subgoal 
+    apply (simp add: Suc3_eq_add_3)
+    using u32_of_u8_list_same
+    by (metis add.commute) 
+  done
+
+
+lemma x64_encode_subl_ri_3 : "
+    and 15 (v >> 4) = 4 \<Longrightarrow> and 15 v \<noteq> 0 \<Longrightarrow>
+    and 3 (k >> 6) = 3 \<Longrightarrow>  and 7 (k >> 3) = 5 \<Longrightarrow>
+    ireg_of_u8 (bitfield_insert_u8 3 (Suc 0) (and 7 k) (and 1 v)) = Some dst \<Longrightarrow>
+    u32_of_u8_list [l ! (pc + 3), l ! (pc + 4), l ! (pc + 5), l ! (pc + 6)] = Some imm \<Longrightarrow>
+    \<not> bit v 3 \<Longrightarrow> \<not> bit v 2 \<Longrightarrow> \<not> bit v (Suc 0) \<Longrightarrow>
+    bitfield_insert_u8 4 4
+     (bitfield_insert_u8 3 (Suc 0) (bitfield_insert_u8 2 (Suc 0) (bitfield_insert_u8 (Suc 0) (Suc 0) 
+       (u8_of_bool (and (u8_of_ireg dst) 8 \<noteq> 0)) 0) 0) 0) 4 \<noteq> 64 \<Longrightarrow>
+    v = bitfield_insert_u8 4 4
+     (bitfield_insert_u8 3 (Suc 0) (bitfield_insert_u8 2 (Suc 0) (bitfield_insert_u8 (Suc 0) (Suc 0) 
+       (u8_of_bool (and (u8_of_ireg dst) 8 \<noteq> 0)) 0) 0) 0) 4 \<and>
+    k = bitfield_insert_u8 6 2 (bitfield_insert_u8 3 3 (and 7 (u8_of_ireg dst)) 5) 3 \<and>
+    [l ! Suc (Suc (Suc pc)), l ! Suc (Suc (Suc (Suc pc))), l ! Suc (Suc (Suc (Suc (Suc pc)))), 
+       l ! Suc (Suc (Suc (Suc (Suc (Suc pc)))))] = u8_list_of_u32 imm
+"
+  apply (simp add: u8_of_ireg_of_u8_iff[symmetric])
+  apply (unfold bitfield_insert_u8_def u8_of_bool_def Let_def )
+  apply simp
+  using encode_subl_ri_4_subgoal_k
+
+  done
